

x	y	z
1	2	13
2	3	18
3	4	23

Let us assume $z = ax + by + c$ is the target equation

$$SSR = \{13 - (a + 2b + c)\}^2 + \{18 - (2a + 3b + c)\}^2 + \{23 - (3a + 4b + c)\}^2$$

$$\frac{dSSR}{da} = 2 \cdot \{13 - (a + 2b + c)\} \cdot (-1) + 2 \cdot \{18 - (2a + 3b + c)\} \cdot (-2) + 2 \cdot \{23 - (3a + 4b + c)\} \cdot (-3)$$

$$\frac{dSSR}{db} = 2 \cdot \{13 - (a + 2b + c)\} \cdot (-2) + 2 \cdot \{18 - (2a + 3b + c)\} \cdot (-3) + 2 \cdot \{23 - (3a + 4b + c)\} \cdot (-4)$$

$$\frac{dSSR}{dc} = 2 \cdot \{13 - (a + 2b + c)\} \cdot (-1) + 2 \cdot \{18 - (2a + 3b + c)\} \cdot (-1) + 2 \cdot \{23 - (3a + 4b + c)\} \cdot (-1)$$

Let $a = 1$, $b = 1$ and $c = 1$

$$\frac{dSSR}{da} = -2 \cdot 1 \cdot \{13 - (1 + 2 \cdot 1 + 1)\} - 2 \cdot 2 \cdot \{18 - (2 \cdot 1 + 3 \cdot 1 + 1)\} - 2 \cdot 3 \cdot \{23 - (3 \cdot 1 + 4 \cdot 1 + 1)\} = -156$$

$$\frac{dSSR}{db} = -2 \cdot 2 \cdot \{13 - (1 + 2 \cdot 1 + 1)\} - 2 \cdot 3 \cdot \{18 - (2 \cdot 1 + 3 \cdot 1 + 1)\} - 2 \cdot 4 \cdot \{23 - (3 \cdot 1 + 4 \cdot 1 + 1)\} = -228$$

$$\frac{dSSR}{dc} = -2 \cdot \{13 - (1 + 2 \cdot 1 + 1)\} - 2 \cdot \{18 - (2 \cdot 1 + 3 \cdot 1 + 1)\} - 2 \cdot \{23 - (3 \cdot 1 + 4 \cdot 1 + 1)\} = -72$$

$$\text{New } a = a - \alpha \cdot \frac{dSSR}{da} \qquad b = b - \alpha \cdot \frac{dSSR}{db} \qquad c = c - \alpha \cdot \frac{dSSR}{dc}$$

$$a = 1 - 0.001(-156) = 1.16$$

$$b = 1 - 0.001(-228) = 1.23$$

$$c = 1 - 0.001(-72) = 1.072$$

$$\frac{dSSR}{da} = -2.1.\{13 - (a + 2b + c)\} - 2.2.\{18 - (2a + 3b + c)\} - 2.3.\{23 - (3a + 4b + c)\}$$

$$\frac{dSSR}{db} = -2.2.\{13 - (a + 2b + c)\} - 2.3.\{18 - (2a + 3b + c)\} - 2.4.\{23 - (3a + 4b + c)\}$$

$$\frac{dSSR}{dc} = -2\{13 - (a + 2b + c)\} - 2\{18 - (2a + 3b + c)\} - 2\{23 - (3a + 4b + c)\}$$

$$a = 1.16 \quad b = 1.23 \quad c = 1.07$$

$$\frac{dSSR}{da} = -2.1.\{13 - (1.16 + 2(1.23) + 1.07)\} - 2.2.\{18 - (2(1.16) + 3(1.23) + 1.07)\} - 2.3.\{23 - (3(1.16) + 4(1.23) + 1.07)\}$$

$$\frac{dSSR}{db} = -2.2.\{13 - (1.16 + 2(1.23) + 1.07)\} - 2.3.\{18 - (2(1.16) + 3(1.23) + 1.07)\} - 2.4.\{23 - (3(1.16) + 4(1.23) + 1.07)\}$$

$$\frac{dSSR}{dc} = -2\{13 - (1.16 + 2(1.23) + 1.07)\} - 2\{18 - (2(1.16) + 3(1.23) + 1.07)\} - 2\{23 - (3(1.16) + 4(1.23) + 1.07)\}$$

$$\text{New } a = 1.16 - 0.001(-141.48) = 1.3 \quad b = 1.23 - 0.001(-207) = 1.44$$

$$c = 1.07 - 0.001(-65.52) = 1.136$$